src/proofs/no_slashable_attestations/supporting_lemmas/ind_inv.dfy
@@ -118,7 +118,7 @@ module Att_Ind_Inv_With_Empty_Init_Att_Slashing_DB
     predicate invs_group_11(dv: DVState)       
     {                
         && inv_exists_att_duty_in_dv_seq_of_att_duty_for_every_slot_in_att_slashing_db_hist(dv)        
-        && inv_db_of_validity_predicate_contains_all_previous_decided_values_c(dv)
+        && inv_latest_attestation_duty_is_from_dv_seq_of_att_duties(dv)
         && inv_exists_att_duty_in_dv_seq_of_att_duty_for_every_slot_in_att_slashing_db_hist_a(dv)        
         && pred_data_of_att_share_is_decided_value(dv)                     
     }
@@ -132,7 +132,7 @@ module Att_Ind_Inv_With_Empty_Init_Att_Slashing_DB
 
     predicate invs_group_13(dv: DVState)       
     {                
-        // && inv_db_of_validity_predicate_contains_all_previous_decided_values_b(dv)    
+        // && inv_queued_att_duties_are_from_dv_seq_of_att_duties(dv)    
         && inv_decided_values_of_previous_duties_are_known_new(dv)    
         && inv_g_d_a(dv)
         && inv_g_d_b(dv)  
